src/StandardLibrary/Validatable.dfy
@@ -1,0 +1,61 @@
+module ExternalInvariants {
+
+  trait {:termination false} Validatable {
+    ghost const Repr: set<Validatable>
+    predicate Valid() 
+      reads this, Repr 
+      ensures Valid() ==> this in Repr
+      ensures Valid() ==> forall v :: v in Repr ==> v.Repr <= Repr
+      ensures Valid() ==> forall v :: v in Repr && v != this ==> this !in v.Repr
+    predicate P() {
+      true
+    }
+
+    twostate lemma AllStillValid() 
+      requires old(AllValid(set v: Validatable | allocated(v) && v.P()))
+      requires Valid()
+      requires forall o :: o !in Repr ==> unchanged(o)
+      requires forall o :: o in Repr ==> o.Valid()
+      ensures AllValid(set v: Validatable | allocated(v) && v.P())
+    {
+      forall v: Validatable | old(allocated(v)) && v.P() ensures v.Valid() {
+        IndependentValidityInductive(v, Repr);
+      }
+    }
+
+    twostate lemma IndependentValidity()
+      requires old(Valid())
+      requires unchanged(this)
+      requires forall v :: v in Repr && v != this ==> v.Valid()
+      ensures Valid()
+  }
+
+  // This is the "external invariant". It must hold as a precondition and postcondition for
+  // every method that crosses the Dafny/external boundary, either incoming or outgoing.
+  // It assumes that the Dafny heap cannot be changed in any other way.
+  // I have to pass in the set of objects implementing Validatable since I can't pass in
+  // "the Dafny heap".
+  predicate AllValid(vs: set<Validatable>) 
+    reads vs
+    reads set v, o | v in vs && o in v.Repr :: o
+  {
+    forall v :: v in vs ==> v.Valid()
+  }
+
+  twostate lemma IndependentValidityInductive(v: Validatable, changed: set<Validatable>)
+      requires old(AllValid(set v': Validatable | allocated(v') && v'.P()))
+      requires forall o :: o !in changed ==> unchanged(o)
+      requires forall o :: o in changed ==> o.Valid()
+      requires allocated(v)
+      decreases v.Repr
+      ensures v.Valid()
+  {
+    assert old(v.Valid());
+    forall v': Validatable | v' in v.Repr && v' != v && old(allocated(v')) ensures v'.Valid() {
+      IndependentValidityInductive(v', changed);
+    }
+    if v !in changed {
+      v.IndependentValidity();
+    }
+  }
+}
